Makefile
@@ -146,6 +146,7 @@ BACKEND=\
   ConstpropOp.v Constprop.v ConstpropOpproof.v Constpropproof.v \
   CSEdomain.v CombineOp.v CSE.v CombineOpproof.v CSEproof.v \
   NeedDomain.v NeedOp.v Deadcode.v Deadcodeproof.v \
+  Unusedglob.v Unusedglobproof.v \
   Machregs.v Locations.v Conventions1.v Conventions.v LTL.v \
   Allocation.v Allocproof.v \
   Tunneling.v Tunnelingproof.v \
@@ -158,8 +159,6 @@ BACKEND=\
   Asm.v Asmgen.v Asmgenproof0.v Asmgenproof1.v Asmgenproof.v \
   Asmrel.v AsmLinking.v \
 
-# Unusedglob.v
-# Unusedglobproof.v
 
 # C front-end modules (in cfrontend/)
 
